wip: extraction of GenNP -> PR reduction

theories/L/Complexity/Cook/FlatGenNP_to_FlatTPR.v
@@ -1,10 +1,9 @@
-From Undecidability.L.Complexity.Cook Require Import Prelim GenNP_PR FlatTPR FlatFinTypes FlatFinTypes_extraction. 
 
-From Undecidability.L.Tactics Require Import LTactics GenEncode.
-From Undecidability.L.Datatypes Require Import LProd LOptions LBool LLNat LLists LSum.
-From Undecidability.L.Complexity Require Import PolyBounds. 
 From Undecidability.L.TM Require Import TMflatEnc TMflat TMEncoding. 
-
+From Undecidability.L.Tactics Require Import LTactics GenEncode.
+From Undecidability.L.Complexity Require Import PolyBounds. 
+From Undecidability.L.Datatypes Require Import LProd LOptions LBool LSum LLNat LLists. 
+From Undecidability.L.Complexity.Cook Require Import Prelim GenNP_PR FlatTPR FlatFinTypes FlatFinTypes_extraction. 
 
 (** * extraction of the reduction from FlatGenNP to FlatPR *)
 
@@ -16,6 +15,9 @@ Hint Resolve fpolarity_enc_correct : Lrewrite.
 
 Run TemplateProgram (tmGenEncode "fpreludeSig'_enc" fpreludeSig').
 Hint Resolve fpreludeSig'_enc_correct : Lrewrite. 
+
+Run TemplateProgram (tmGenEncode "delim_enc" delim). 
+Hint Resolve delim_enc_correct : Lrewrite.
 
 Run TemplateProgram (tmGenEncode "evalEnv_enc" (evalEnv nat nat nat nat)).
 Hint Resolve evalEnv_enc_correct : Lrewrite. 
@@ -49,6 +51,64 @@ Proof.
   extract. solverec. unfold c__stateEnv. solverec. 
 Defined. 
 
+(**extraction of type constructors *)
+
+Definition c__flatStateSigma := 13.
+Instance term_flatStateSigma : computableTime' flatStateSigma (fun tm _ => (c__flatStateSigma, tt)). 
+Proof. 
+  extract. solverec. 
+  unfold c__flatStateSigma; lia.
+Defined. 
+
+Definition c__flatPolSigma := c__mult1 + c__flatStateSigma + 1 + c__mult * (flatPolarity + 1).
+Definition flatPolSigma_time tm := (flatStateSigma tm + 1) * c__flatPolSigma.
+Instance term_flatPolSigma : computableTime' flatPolSigma (fun tm _ => (flatPolSigma_time tm, tt)). 
+Proof. 
+  extract. solverec. 
+  unfold mult_time. unfold flatPolSigma_time, c__flatPolSigma. solverec. 
+Defined. 
+
+Definition c__flatTapeSigma := c__add1 + 1 + (flatDelim + 1) * c__add.
+Definition flatTapeSigma_time (tm : TM) := flatPolSigma_time tm + c__flatTapeSigma.
+Instance term_flatTapeSigma : computableTime' flatTapeSigma (fun tm _ => (flatTapeSigma_time tm, tt)). 
+Proof. 
+  extract. solverec. 
+  unfold add_time. unfold flatTapeSigma_time, c__flatTapeSigma. solverec. 
+Defined. 
+
+Definition c__flatStates := c__mult1 + c__flatStateSigma + 10.
+Definition flatStates_time (tm : TM) := mult_time (states tm) (flatStateSigma tm) + c__flatStates.
+Instance term_flatStates : computableTime' flatStates (fun tm _ => (flatStates_time tm, tt)).
+Proof. 
+  extract. solverec. 
+  unfold flatStates_time, c__flatStates. solverec.  
+Defined. 
+
+Definition c__flatGamma := c__add1 + 1.
+Definition flatGamma_time (tm : TM) := flatStates_time tm + flatTapeSigma_time tm + add_time (flatStates tm) + c__flatGamma.
+Instance term_flatGamma : computableTime' flatGamma (fun tm _ => (flatGamma_time tm, tt)). 
+Proof. 
+  extract. solverec. 
+  unfold flatGamma_time, c__flatGamma; solverec. 
+Defined. 
+
+Definition c__flatPreludeSig' :=c__add1 + 5 * c__add + 22.
+Instance term_flatPreludeSig' : computableTime' flatPreludeSig' (fun tm _ => (c__flatPreludeSig', tt)). 
+Proof. 
+  extract. solverec. 
+  unfold add_time. unfold c__flatPreludeSig', flatSome. solverec.
+Defined. 
+
+Definition c__flatAlphabet := c__add1 + c__flatPreludeSig' + 1.
+Definition flatAlphabet_time (tm : TM) := flatGamma_time tm + add_time (flatGamma tm) + c__flatAlphabet.
+Instance term_flatAlphabet : computableTime' flatAlphabet (fun tm _ => (flatAlphabet_time tm, tt)). 
+Proof. 
+  extract. solverec. 
+  unfold flatAlphabet_time, c__flatAlphabet. solverec. 
+Defined. 
+  
+(** flattenPolarity *)
+
 Definition c__flattenPolarity := 11.
 Instance term_flattenPolarity : computableTime' flattenPolarity (fun p _ => (c__flattenPolarity, tt)). 
 Proof. 
@@ -57,6 +117,7 @@ Proof.
   eapply (computableTimeExt H).
   extract. solverec. all: now unfold c__flattenPolarity.
 Defined.
+
 
 (*define notations again, because Coq doesn't allow to keep notations beyond the end of a section (why!?) *)
 Notation fpolSigma  := (prod fpolarity fstateSigma).
@@ -88,6 +149,11 @@ Section fix_option_map.
     extract. solverec. 
     all: unfold optionMap_time, c__optionMap; solverec. 
   Defined. 
+
+  Lemma optionMap_time_bound_c (a : option A) c : optionMap_time (fun _ => c) a <= c + c__optionMap. 
+  Proof. 
+    destruct a; cbn; lia. 
+  Qed. 
 End fix_option_map. 
 
 (*reifyStateSigmaFlat *)
@@ -104,8 +170,6 @@ Proof.
   2: unfold optionMap_time; destruct nth_error. 
   all: unfold reifyStateSigmaFlat_time, c__reifyStateSigmaFlat; solverec. 
 Defined. 
-
-
 
 (*optBind & optReturn*)
 Section fix_optBind.
@@ -125,76 +189,606 @@ Section fix_optBind.
     extract. solverec. 
   Defined. 
 End fix_optBind. 
-  
-Definition test := fun (flatTM : TM) (env : evalEnvFlat) (c : fpolSigma) =>
-   let (p, s) := c in
-   match reifyPolarityFlat env p with
-   | Some x =>
-       match reifyStateSigmaFlat env s with
-       | Some x0 =>
-           optReturn (flatPair flatPolarity (flatOption (sig flatTM)) x x0)
-       | None => None
-       end
-   | None => None
-   end. 
 
-From Undecidability.L.TM Require Import TMflatEnc TMflat TMEncoding. 
+(** reifyPolSigmaFlat *)
 
-Require Import Undecidability.L.Tactics.ComputableTactics.
-Import ComputableTactics.Intern.
-Definition reifyPolSigmaFlat_time (env : evalEnvFlat) (c : fpolSigma) := 1. 
-Instance term_test : computableTime' test (fun tm _ => (1, fun env _ => (1, fun c _ => (reifyPolSigmaFlat_time env c, tt)))).
-Proof.
-  unfold test. extract. extractAs t. computable_using_noProof t. cstep.
-  cstep. cstep. cstep. cstep. cstep. cstep. unfold optReturn. cstep. 2: cstep. 
-
-Instance term_reifyPolSigmaFlat : computableTime' reifyPolSigmaFlat (fun tm _ => (1, fun env _ => (1, fun c _ => (reifyPolSigmaFlat_time env c, tt)))). 
+Definition c__reifyPolSigmaFlat := 32. 
+Definition reifyPolSigmaFlat_time sig (env : evalEnvFlat) (c : fpolSigma) := 
+  let (p, s) := c in reifyPolarityFlat_time env p + reifyStateSigmaFlat_time env s + 
+    match reifyPolarityFlat env p, reifyStateSigmaFlat env s with 
+    | Some a, Some b  => flatPair_time a (flatOption sig)
+    | _,_ => 0
+    end + c__reifyPolSigmaFlat.
+Instance term_reifyPolSigmaFlat : computableTime' reifyPolSigmaFlat (fun tm _ => (1, fun env _ => (1, fun c _ => (reifyPolSigmaFlat_time (sig tm) env c, tt)))). 
 Proof. 
   unfold reifyPolSigmaFlat. unfold optBind. 
+  extract. intros tm _. split; [solverec | ]. 
+  intros env ?. split; [solverec | ]. 
+  intros [p s] ?. unfold reifyPolSigmaFlat_time. cbn. solverec. 
+  all: unfold flatStateSigma, c__reifyPolSigmaFlat; solverec. 
+Defined. 
+
+(** reifyTapeSigmaFlat *)
+Definition c__reifyTapeSigmaFlat := c__optionMap + 35. 
+Definition reifyTapeSigmaFlat_time (sig : nat) (env : evalEnvFlat) (c : ftapeSigma) := 
+  match c with 
+  | inl _ => 0 
+  | inr c => reifyPolSigmaFlat_time sig env c
+  end + c__reifyTapeSigmaFlat.
+Instance term_reifyTapeSigmaFlat : computableTime' reifyTapeSigmaFlat (fun tm _ => (1, fun env _ => (1, fun c _ => (reifyTapeSigmaFlat_time (sig tm) env c, tt)))). 
+Proof. 
+  extract. unfold reifyTapeSigmaFlat_time. 
+  intros tm _. split; [solverec | ]. 
+  intros env ?. split; [solverec | ]. 
+  intros [ c | c] ?. 
+  - unfold c__reifyTapeSigmaFlat. solverec. 
+  - cbn -[c__reifyTapeSigmaFlat]. rewrite optionMap_time_bound_c. split; [unfold c__reifyTapeSigmaFlat; nia| easy]. 
+Defined. 
+
+(** reifyStatesFlat *)
+Definition c__reifyStatesFlat := 32 + c__stateEnv + c__flatStateSigma.
+Definition reifyStatesFlat_time (sig : nat) (env : evalEnvFlat) (c : fStates) :=   
+  let (s, c) := c in nth_error_time (stateEnv env) s + reifyStateSigmaFlat_time env c + 
+  match nth_error (stateEnv env) s with 
+  | Some s => flatPair_time s (flatOption sig) 
+  | _ => 0
+  end + c__reifyStatesFlat.
+Instance term_reifyStatesFlat : computableTime' reifyStatesFlat (fun tm _ => (1, fun env _ => (1, fun c _ => (reifyStatesFlat_time (sig tm) env c, tt)))). 
+Proof. 
+  unfold reifyStatesFlat, optBind. 
+  extract. unfold reifyStatesFlat_time, c__reifyStatesFlat, flatStateSigma; solverec. 
+  - now inv H. 
+  - now inv H. 
+Defined. 
+ 
+(** reifyGammaFlat *)
+Definition c__reifyGammaFlat := 8 + c__add1 + c__optionMap.
+Definition reifyGammaFlat_time (tm : TM) (env : evalEnvFlat) (c : fGamma) := 
+  match c with 
+  | inl c => reifyStatesFlat_time (sig tm) env c 
+  | inr c => flatStates_time tm + reifyTapeSigmaFlat_time (sig tm) env c + add_time (flatStates tm)
+  end + c__reifyGammaFlat.
+Instance term_reifyGammaFlat : computableTime' reifyGammaFlat (fun tm _ => (1, fun env _ => (1, fun c _ => (reifyGammaFlat_time tm env c, tt)))). 
+Proof. 
+  extract. 
+  intros tm _. split; [solverec | ]. 
+  intros env ?. split; [solverec | ]. 
+  intros [c | c]; (split; [ |easy ]). 
+  - cbn. rewrite optionMap_time_bound_c. lia.
+  - cbn -[Nat.mul Nat.add].
+    rewrite optionMap_time_bound_c. 
+    unfold reifyGammaFlat_time, c__reifyGammaFlat. nia. 
+Defined. 
+
+(** flatNsig *)
+Definition c__flatNsig := c__add1 + 5 * c__add + 13.
+Instance term_flatNsig : computableTime' flatNsig (fun n _ => (c__flatNsig, tt)). 
+Proof. 
+  extract. solverec. unfold add_time. cbn. easy.
+Defined. 
+
+(** reifyPreludeSig'Flat *)
+Definition c__reifyPreludeSigPFlat := 8 + c__sigmaEnv + c__flatNsig + 18.
+Definition reifyPreludeSig'Flat_time (env : evalEnvFlat) (c : fpreludeSig') :=  
+  match c with fnsigVar n => nth_error_time (sigmaEnv env) n | _ => 0 end + c__reifyPreludeSigPFlat.
+Instance term_reifyPreludeSig'Flat : computableTime' reifyPreludeSig'Flat (fun env _ => (1, fun c _ => (reifyPreludeSig'Flat_time env c, tt))).
+Proof. 
+  unfold reifyPreludeSig'Flat, optBind. 
   extract. solverec. 
+  all: unfold reifyPreludeSig'Flat_time, c__reifyPreludeSigPFlat; solverec. 
+Defined. 
+  
+(** reifyAlphabetFlat *) 
+Definition c__reifyAlphabetFlat := c__add1 + 7 + c__optionMap.
+Definition reifyAlphabetFlat_time (tm : TM) (env : evalEnvFlat) (c : fAlphabet) := 
+  match c with 
+  | inl s => reifyGammaFlat_time tm env s
+  | inr s => flatGamma_time tm + reifyPreludeSig'Flat_time env s + add_time (flatGamma tm)
+  end + c__reifyAlphabetFlat.
+Instance term_reifyAlphabetFlat : computableTime' reifyAlphabetFlat (fun tm _ => (1, fun env _ => (1, fun c _ => (reifyAlphabetFlat_time tm env c, tt)))).
+Proof. 
+  extract. 
+  intros tm _; split;[solverec | ]. 
+  intros env ?; split; [solverec | ]. 
+  intros [s | s] ?; (split; [ | easy]).
+  - cbn. rewrite optionMap_time_bound_c. nia.  
+  - solverec. rewrite optionMap_time_bound_c. 
+    unfold reifyAlphabetFlat_time, c__reifyAlphabetFlat. solverec. 
+Defined. 
 
 
+(** reifyWindowFlat *)
+Definition reifyWindowFlat (tm : TM) := reifyWindow (reifyAlphabetFlat tm). 
+Definition c__reifyWindow := 60. 
+Definition reifyWindow_time (tm : TM) (env : evalEnvFlat) (win : TPRWin fAlphabet) := 
+  let '{winEl1, winEl2, winEl3} / {winEl4, winEl5, winEl6} := win in 
+  reifyAlphabetFlat_time tm env winEl1 + reifyAlphabetFlat_time tm env winEl2 + reifyAlphabetFlat_time tm env winEl3 +
+  reifyAlphabetFlat_time tm env winEl4 + reifyAlphabetFlat_time tm env winEl5 + reifyAlphabetFlat_time tm env winEl6
+  + c__reifyWindow.
+Instance term_reifyWindow : computableTime' reifyWindowFlat (fun tm _ => (1, fun env _ => (1, fun win _ => (reifyWindow_time tm env win, tt)))).
+Proof. 
+  unfold reifyWindowFlat, reifyWindow, optBind.
+  extract. solverec. 
+  all: unfold c__reifyWindow; solverec. 
+Defined. 
 
-  Definition reifyPolSigmaFlat (env : evalEnvFlat) (c : fpolSigma) :=
-    match c with
-    | (p, s) => do p <- reifyPolarityFlat env p;
-                do s <- reifyStateSigmaFlat env s;
-                optReturn (flatPair flatPolarity flatStateSigma p s)
-    end. 
+(** listProd *)
+Section fixListProd. 
+  Variable (X : Type).
+  Context `{intX : registered X}.
 
-  Definition reifyTapeSigmaFlat (env : evalEnvFlat) (c : ftapeSigma) :=
-    match c with
-    | inl delimC => Some (flatDelimC)
-    | inr c => option_map (flatInr flatDelim) (reifyPolSigmaFlat env c)
-    end.
+  Definition c__listProd1 := 17 + c__map. 
+  Definition c__listProd2 := 18. 
+  Fixpoint list_prod_time (l1 : list X) (l2 : list (list X)) := 
+    match l1 with 
+    | [] => 0
+    | (a :: l1) => (|l2| + 1) * c__listProd1 + list_prod_time l1 l2
+    end + c__listProd2. 
+  Global Instance term_listProd : computableTime' (@list_prod X) (fun l1 _ => (5, fun l2 _ => (list_prod_time l1 l2, tt))). 
+  Proof. 
+    extract. 
+    solverec. 
+    2: rewrite map_time_const, map_length.
+    all: unfold c__listProd1, c__listProd2; solverec. 
+  Defined. 
 
-  Definition reifyStatesFlat (env : evalEnvFlat) (c : fStates) :=
-    match c with
-    | (v, s) => do p <- nth_error (stateEnv env) v;
-                do s <- reifyStateSigmaFlat env s;
-                optReturn (flatPair flatstates flatStateSigma p s)
-    end. 
+  Lemma list_prod_length (l1 : list X) l2 : |list_prod l1 l2| = |l1| * |l2|.
+  Proof. 
+    unfold list_prod. induction l1; cbn; [easy | ].
+    rewrite app_length, IHl1, map_length. lia. 
+  Qed. 
+End fixListProd. 
 
-  Definition reifyGammaFlat (env : evalEnvFlat) (c : fGamma) :=
-    match c with
-    | inl s => option_map (flatInl) (reifyStatesFlat env s)
-    | inr c => option_map (flatInr flatStates) (reifyTapeSigmaFlat env c)
-    end. 
+(** mkVarEnv_step *)
+Definition mkVarEnv_step (l : list nat) (acc : list (list nat)) := list_prod l acc ++ acc. 
+Definition c__mkVarEnvStep := 16. 
+Definition mkVarEnv_step_time (l : list nat) (acc : list (list nat)) := list_prod_time l acc + (|l| * |acc| * c__mkVarEnvStep) + c__mkVarEnvStep.
+Instance term_mkVarEnv_step : computableTime' mkVarEnv_step (fun l1 _ => (1, fun l2 _ => (mkVarEnv_step_time l1 l2, tt))). 
+Proof. 
+  extract. solverec. 
+  rewrite list_prod_length. 
+  unfold mkVarEnv_step_time, c__mkVarEnvStep. solverec. 
+Defined. 
 
-  Definition reifyPreludeSig'Flat (env : evalEnvFlat) (c : fpreludeSig') := 
-    match c with
-    | fnblank => optReturn flatNblank
-    | fnstar => optReturn flatNstar
-    | fninit => optReturn flatNinit
-    | fndelimC => optReturn flatNdelimC
-    | fnsigVar n => do s <- nth_error (sigmaEnv env) n;
-                    optReturn (flatNsig s)
-    end. 
+(** it *)
+Section fixIt. 
+  Variable (X : Type). 
+  Context `{intX : registered X}.
 
-  Definition reifyAlphabetFlat (env : evalEnvFlat) (c : fAlphabet) := 
-    match c with 
-    | inl s => option_map (flatInl) (reifyGammaFlat env s)
-    | inr s => option_map (flatInr flatGamma) (reifyPreludeSig'Flat env s) 
-  end.  
+  Definition c__it := 10.
+  Fixpoint it_time f (fT: X -> nat) (n : nat) (acc : X) :=   
+  match n with 
+  | 0 => 0 
+  | S n => fT (it f n acc) + it_time f fT n acc 
+  end + c__it.
+  Global Instance term_it : computableTime' (@it X) (fun f fT => (5, fun n _ => (5, fun acc _ => (it_time f (callTime fT) n acc, tt)))).
+  Proof. 
+    extract. solverec. all: unfold c__it. 
+    - lia. 
+    - fold (it x). solverec. 
+  Defined.  
+End fixIt. 
+
+(** mkVarEnv *)
+Definition c__mkVarEnv := 14.
+Definition mkVarEnv_time (l : list nat) (n : nat) := it_time (mkVarEnv_step l) (mkVarEnv_step_time l) n [[]] + c__mkVarEnv.
+Instance term_mkVarEnv : computableTime' (@mkVarEnv nat) (fun l _ => (1, fun n _ => (mkVarEnv_time l n, tt))). 
+Proof.  
+  apply computableTimeExt with (x := fun l n => it (mkVarEnv_step l) n [[]]). 
+  1: { unfold mkVarEnv, mkVarEnv_step. easy. }
+  extract. solverec.  
+  unfold mkVarEnv_time. change (fun x => ?h x) with h. 
+  now unfold c__mkVarEnv. 
+Defined. 
+
+Fact mkVarEnv_length (l : list nat) n : |mkVarEnv l n|  = (|l| + 1) ^ n.
+Proof. 
+  unfold mkVarEnv. induction n; cbn; [easy | ].
+  rewrite app_length, list_prod_length. rewrite IHn. 
+  nia. 
+Qed.
+
+(** tupToEvalEnv *)
+Definition c__tupToEvalEnv := 17.
+Instance term_tupToEvalEnv : computableTime' (@tupToEvalEnv nat nat nat nat) (fun p _ => (c__tupToEvalEnv, tt)). 
+Proof. 
+  extract. solverec. 
+  now unfold c__tupToEvalEnv. 
+Defined.
+
+(** seq *)
+Definition c__seq := 20.
+Definition seq_time (len : nat) := (len + 1) * c__seq.
+Instance term_seq : computableTime' seq (fun start _ => (5, fun len _ => (seq_time len, tt))). 
+Proof. 
+  extract. solverec. 
+  all: unfold seq_time, c__seq; solverec. 
+Defined. 
+
+(** prodLists *)
+Section fixprodLists. 
+  Variable (X Y : Type).
+  Context `{Xint : registered X} `{Yint : registered Y}.
+
+  Definition c__prodLists1 := 22 + c__map. 
+  Definition c__prodLists2 := 1 + c__map + 16.
+  Fixpoint prodLists_time (l1 : list X) (l2 : list Y) := 
+    match l1 with 
+    | [] => 0 
+    | _ :: l1 => (|l2|) * c__prodLists2 + prodLists_time l1 l2 
+    end + c__prodLists1. 
+  Global Instance term_prodLists : computableTime' (@prodLists X Y) (fun l1 _ => (5, fun l2 _ => (prodLists_time l1 l2, tt))). 
+  Proof. 
+    apply computableTimeExt with (x := fix rec (A : list X) (B : list Y) : list (X * Y) := 
+      match A with 
+      | [] => []
+      | x :: A' => map (@pair X Y x) B ++ rec A' B 
+      end). 
+    1: { unfold prodLists. change (fun x => ?h x) with h. intros l1 l2. induction l1; easy. }
+    extract. solverec. 
+    all: unfold c__prodLists1, c__prodLists2; solverec. 
+    rewrite map_length, map_time_const. solverec. 
+  Defined. 
+End fixprodLists. 
+
+(** makeAllEvalEnvFlat *)
+Definition c__makeAllEvalEnvFlat1 := c__flatStateSigma + c__map + 59.
+Definition c__makeAllEvalEnvFlat2 := c__tupToEvalEnv + c__map. 
+Definition makeAllEvalEnvFlat_time (tm : TM) (n1 n2 n3 n4 : nat) := 
+  seq_time flatPolarity 
+  + seq_time (sig tm)
+  + seq_time (flatStateSigma tm)
+  + seq_time (states tm)
+  + mkVarEnv_time (seq 0 flatPolarity) n1 
+  + mkVarEnv_time (seq 0 (sig tm)) n2
+  + mkVarEnv_time (seq 0 (flatStateSigma tm)) n3
+  + mkVarEnv_time (seq 0 (states tm)) n4
+  + prodLists_time (mkVarEnv (seq 0 flatPolarity) n1) (mkVarEnv (seq 0 (sig tm)) n2)
+  + prodLists_time (prodLists (mkVarEnv (seq 0 flatPolarity) n1) (mkVarEnv (seq 0 (sig tm)) n2)) (mkVarEnv (seq 0 (flatStateSigma tm)) n3)
+  + prodLists_time (prodLists (prodLists (mkVarEnv (seq 0 flatPolarity) n1) (mkVarEnv (seq 0 (sig tm)) n2)) (mkVarEnv (seq 0 (flatStateSigma tm)) n3)) (mkVarEnv (seq 0 (states tm)) n4) 
+  + (4^n1) * ((sig tm + 1) ^n2) * ((flatStateSigma tm + 1) ^n3) * ((states tm + 1) ^ n4) * c__makeAllEvalEnvFlat2
+  + c__makeAllEvalEnvFlat1.
+
+Instance term_makeAllEvalEnvFlat : computableTime' makeAllEvalEnvFlat (fun tm _ => (1, fun n1 _ => (1, fun n2 _ => (1, fun n3 _ => (1, fun n4 _ => (makeAllEvalEnvFlat_time tm n1 n2 n3 n4, tt)))))). 
+Proof. 
+  unfold makeAllEvalEnvFlat, makeAllEvalEnv. 
+  extract. 
+  solverec. 
+  rewrite map_time_const. 
+  rewrite !prodLists_length, !mkVarEnv_length, !seq_length.
+  cbn [length Nat.add]. 
+  rewrite !seq_length. 
+  unfold makeAllEvalEnvFlat_time, c__makeAllEvalEnvFlat1, c__makeAllEvalEnvFlat2. unfold flatStateSigma, flatOption. solverec. 
+  replace (1 + (sig x + 1)) with (1 + sig x + 1) by lia. 
+  leq_crossout.
+Defined. 
+
+(** filterSome *)
+Section fixfilterSome.
+  Variable (X : Type).
+  Context `{intX : registered X}.
+  Definition c__filterSome := 16. 
+  Definition filterSome_time (l : list (option X)) := (|l| + 1) * c__filterSome.
+  Global Instance term_filterSome : computableTime' (@filterSome X) (fun l _ => (filterSome_time l, tt)). 
+  Proof. 
+    apply computableTimeExt with (x := fix rec (l : list (option X)) :=  
+      match l with 
+      | [] => []
+      | Some x :: l => x :: rec l
+      | None :: l => rec l
+      end). 
+    1: { unfold filterSome. intros l. induction l; cbn; [ | destruct a]; easy. }
+    extract. solverec. 
+    all: unfold filterSome_time, c__filterSome; solverec. 
+  Defined. 
+End fixfilterSome.
+
+(** makeRules'_flat_step *)
+Definition makeRules'_flat_step tm win (env : evalEnvFlat) := reifyWindowFlat tm env win.
+
+Definition c__makeRulesPFlatStep := 3.
+Definition makeRules'_flat_step_time (tm : TM) (win : TPRWin fAlphabet) (env : evalEnvFlat) := reifyWindow_time tm env win + c__makeRulesPFlatStep.
+Instance term_makeRules'_flat_step : computableTime' makeRules'_flat_step (fun tm _ => (1, fun win _ => (1, fun env _ => (makeRules'_flat_step_time tm win env, tt)))). 
+Proof. 
+  extract. solverec. 
+  unfold makeRules'_flat_step_time, c__makeRulesPFlatStep; solverec. 
+Defined. 
+
+(** makeRules' *)
+Definition makeRules'_flat (tm : TM) := makeRules' (reifyAlphabetFlat tm). 
+Definition c__makeRules' := 4.
+Definition makeRules'_flat_time (tm : TM) (envs : list evalEnvFlat) (win : TPRWin fAlphabet) := map_time (fun env => makeRules'_flat_step_time tm win env) envs + (|envs| + 1) * c__filterSome + c__makeRules'.
+Instance term_makeRules' : computableTime' makeRules'_flat (fun tm _ => (1, fun envs _ => (1, fun win _ => (makeRules'_flat_time tm envs win, tt)))). 
+Proof. 
+  unfold makeRules'_flat, makeRules'. 
+  apply computableTimeExt with (x := fun tm l win => filterSome (map (makeRules'_flat_step tm win) l)). 
+  1: { unfold makeRules'_flat_step, reifyWindowFlat. easy. }
+  extract. solverec. 
+  unfold filterSome_time. rewrite map_length. 
+  unfold makeRules'_flat_time, c__makeRules'.
+  nia. 
+Defined. 
+
+(** makeRulesFlat *)
+Definition c__makeRulesFlat := 4.
+Definition makeRulesFlat_time (tm : TM) (envs : list evalEnvFlat) (windows : list (TPRWin fAlphabet)) := map_time (makeRules'_flat_time tm envs) windows + concat_time (map (makeRules'_flat tm envs) windows) + c__makeRulesFlat.
+Instance term_makeRulesFlat : computableTime' makeRulesFlat (fun tm _ => (1, fun envs _ => (1, fun wins _ => (makeRulesFlat_time tm envs wins, tt)))). 
+Proof. 
+  unfold makeRulesFlat, makeRules. 
+  apply computableTimeExt with (x := fun tm allEnv rules => concat (map (makeRules'_flat tm allEnv) rules)). 
+  1: { unfold makeRules'_flat. easy. }
+  extract. solverec. 
+  unfold makeRulesFlat_time, c__makeRulesFlat. solverec.  
+Defined. 
+
+(**envAddState *)
+Definition c__envAddState := c__polarityEnv + c__sigmaEnv + c__stateSigmaEnv + c__stateEnv + 7.
+Instance term_envAddState : computableTime' (@envAddState nat nat nat nat) (fun q _ => (1, fun env _ => (c__envAddState, tt))). 
+Proof. 
+  extract. solverec. 
+  unfold c__envAddState. lia. 
+Defined. 
+
+(** envAddSSigma *)
+Definition c__envAddSSigma := c__polarityEnv + c__sigmaEnv + c__stateSigmaEnv + c__stateEnv + 7.
+Instance term_envAddSSigma : computableTime' (@envAddSSigma nat nat nat nat) (fun m _ => (1, fun env _ => (c__envAddSSigma, tt))). 
+Proof. 
+  extract. solverec. 
+  unfold c__envAddSSigma. lia. 
+Defined. 
+
+(** transEnvAddS *)
+Definition c__transEnvAddS := 2* c__envAddState + 3.
+Instance term_transEnvAddS : computableTime' (@transEnvAddS nat nat nat nat) (fun q _ => (1, fun q' _ => (1, fun env _ => (c__transEnvAddS, tt)))). 
+Proof. 
+  extract. solverec. 
+  unfold c__transEnvAddS. lia. 
+Defined. 
+
+(** transEnvAddSM *)
+Definition c__transEnvAddSM := c__transEnvAddS + 2 * c__envAddSSigma + 5.
+Instance term_transEnvAddSM : computableTime' (@transEnvAddSM nat nat nat nat) (fun q _ => (1, fun q' _ => (1, fun m _ => (1, fun m' _ => (1, fun env _ => (c__transEnvAddSM, tt)))))).
+Proof. 
+  extract. solverec. 
+  unfold c__transEnvAddSM; lia. 
+Defined. 
 
 
+(** tape windows *)
+Definition c__flatMTRWindows := 22.
+Definition flatMTRWindows_time (tm : TM) := makeAllEvalEnvFlat_time tm 1 4 0 0 + makeRulesFlat_time tm (makeAllEvalEnvFlat tm 1 4 0 0) mtrRules + c__flatMTRWindows.
+Instance term_flatMTRWindows : computableTime' flatMTRWindows (fun tm _ => (flatMTRWindows_time tm, tt)). 
+Proof. 
+  extract. recRel_prettify2. 
+  unfold flatMTRWindows_time, c__flatMTRWindows. unfold flatSome. lia. 
+Defined. 
+
+Definition c__flatMTIWindows := 25. 
+Definition flatMTIWindows_time (tm : TM) := makeAllEvalEnvFlat_time tm 2 0 4 0 + makeRulesFlat_time tm (makeAllEvalEnvFlat tm 2 0 4 0) mtiRules + c__flatMTIWindows.
+Instance term_flatMTIWindows : computableTime' flatMTIWindows (fun tm _ => (flatMTIWindows_time tm, tt)). 
+Proof. 
+  extract. recRel_prettify2. 
+  unfold flatMTIWindows_time, c__flatMTIWindows. unfold flatSome. lia. 
+Defined. 
+
+Definition c__flatMTLWindows := 22. 
+Definition flatMTLWindows_time (tm : TM) := makeAllEvalEnvFlat_time tm 1 4 0 0 + makeRulesFlat_time tm (makeAllEvalEnvFlat tm 1 4 0 0) mtlRules + c__flatMTLWindows.
+Instance term_flatMTLWindows : computableTime' flatMTLWindows (fun tm _ => (flatMTLWindows_time tm, tt)). 
+Proof. 
+  extract. recRel_prettify2.  
+  unfold flatMTLWindows_time, c__flatMTLWindows. unfold flatSome. lia. 
+Defined. 
+
+Definition c__flatTapeWindows := 19. 
+Definition flatTapeWindows_time (tm : TM) := flatMTRWindows_time tm + flatMTIWindows_time tm + flatMTLWindows_time tm + (|flatMTIWindows tm| + |flatMTRWindows tm| + 1) * c__flatTapeWindows.
+Instance term_flatTapeWindows : computableTime' flatTapeWindows (fun tm _ => (flatTapeWindows_time tm, tt)). 
+Proof. 
+  extract. recRel_prettify2. 
+  unfold flatTapeWindows_time, c__flatTapeWindows. nia.
+Defined. 
+  
+(** non-halting state windows *)
+(** makeSome_base *)
+Definition makeSome_base_flat (tm : TM) (windows : list (TPRWin fAlphabet)) (q q' m m' : nat):= @makeSome_base nat nat nat nat nat windows q q' m m' (makeRulesFlat tm).
+
+Definition c__makeSomeBaseFlat1 := c__transEnvAddSM + c__map.
+Definition c__makeSomeBaseFlat2 := c__map + 8.
+Definition makeSome_base_flat_time (tm : TM) (windows : list (TPRWin fAlphabet)) (q q' m m' : nat) (envs : list evalEnvFlat) := (|envs|) * c__makeSomeBaseFlat1+ makeRulesFlat_time tm (map (transEnvAddSM q q' m m') envs) windows + c__makeSomeBaseFlat2.
+Instance term_makeSome_base_flat : computableTime' makeSome_base_flat (fun tm _ => (1, fun windows _ => (1, fun q _ => (1, fun q' _ => (1, fun m _ => (1, fun m' _ => (1, fun envs _ => (makeSome_base_flat_time tm windows q q' m m' envs, tt)))))))). 
+Proof. 
+  unfold makeSome_base_flat, makeSome_base.
+  extract. solverec. 
+  rewrite map_time_const. 
+  unfold makeSome_base_flat_time, c__makeSomeBaseFlat1, c__makeSomeBaseFlat2. 
+  Set Printing All. unfold evalEnvFlat. nia.
+Defined. 
+
+(** makeSomeRight *)
+Definition makeSomeRightFlat tm q q' m m' := makeSomeRight q q' m m' (makeRulesFlat tm). 
+Definition c__makeSomeRightFlat := 7.
+Instance term_makeSomeRightFlat : computableTime' makeSomeRightFlat (fun tm _ => (1, fun q _ => (1, fun q' _ => (1, fun m _ => (1, fun m' _ => (c__makeSomeRightFlat, fun envs _ => (makeSome_base_flat_time tm makeSomeRight_rules q q' m m' envs, tt))))))).
+Proof. 
+  unfold makeSomeRightFlat, makeSomeRight.
+  apply computableTimeExt with (x := fun tm q q' m m' => makeSome_base_flat tm makeSomeRight_rules q q' m m'). 
+  1: { unfold makeSome_base_flat. easy. }
+  extract. solverec. 
+  now unfold c__makeSomeRightFlat. 
+Defined. 
+  
+(** makeSomeLeft *)
+Definition makeSomeLeftFlat tm q q' m m' := makeSomeLeft q q' m m' (makeRulesFlat tm). 
+Definition c__makeSomeLeftFlat := 7.
+Instance term_makeSomeLeftFlat : computableTime' makeSomeLeftFlat (fun tm _ => (1, fun q _ => (1, fun q' _ => (1, fun m _ => (1, fun m' _ => (c__makeSomeLeftFlat, fun envs _ => (makeSome_base_flat_time tm makeSomeLeft_rules q q' m m' envs, tt))))))).
+Proof. 
+  unfold makeSomeLeftFlat, makeSomeLeft.
+  apply computableTimeExt with (x := fun tm q q' m m' => makeSome_base_flat tm makeSomeLeft_rules q q' m m'). 
+  1: { unfold makeSome_base_flat. easy. }
+  extract. solverec. 
+  now unfold c__makeSomeLeftFlat. 
+Defined. 
+
+(**makeSomeStay *)
+Definition makeSomeStayFlat tm q q' m m' := makeSomeStay q q' m m' (makeRulesFlat tm). 
+Definition c__makeSomeStayFlat := 7.
+Instance term_makeSomeStayFlat : computableTime' makeSomeStayFlat (fun tm _ => (1, fun q _ => (1, fun q' _ => (1, fun m _ => (1, fun m' _ => (c__makeSomeStayFlat, fun envs _ => (makeSome_base_flat_time tm makeSomeStay_rules q q' m m' envs, tt))))))).
+Proof. 
+  unfold makeSomeStayFlat, makeSomeStay.
+  apply computableTimeExt with (x := fun tm q q' m m' => makeSome_base_flat tm makeSomeStay_rules q q' m m'). 
+  1: { unfold makeSome_base_flat. easy. }
+  extract. solverec. 
+  now unfold c__makeSomeStayFlat. 
+Defined. 
+
+(** makeNone_base *)
+Definition makeNone_base_flat (tm : TM) (windows : list (TPRWin fAlphabet)) (q q' : nat) := @makeNone_base nat nat nat nat nat windows q q' (makeRulesFlat tm). 
+Definition c__makeNoneBaseFlat1 := c__transEnvAddS + c__map.
+Definition c__makeNoneBaseFlat2 := c__map + 6.
+Definition makeNone_base_flat_time (tm : TM) (rules :list (TPRWin fAlphabet)) (q q' : nat) (envs : list evalEnvFlat) := (|envs|) * c__makeNoneBaseFlat1 + makeRulesFlat_time tm (map (transEnvAddS q q') envs) rules + c__makeNoneBaseFlat2.
+Instance term_makeNone_base_flat : computableTime' makeNone_base_flat (fun tm _ => (1, fun rules _ => (1, fun q _ => (1, fun q' _ => (1, fun envs _ => (makeNone_base_flat_time tm rules q q' envs, tt)))))). 
+Proof. 
+  unfold makeNone_base_flat, makeNone_base. 
+  extract. solverec. 
+  rewrite map_time_const.
+  unfold makeNone_base_flat_time, c__makeNoneBaseFlat1, c__makeNoneBaseFlat2. 
+  Set Printing All. unfold evalEnvFlat. nia. 
+Defined. 
+
+(** makeNoneRight *)
+Definition makeNoneRightFlat tm q q' := makeNoneRight q q' (makeRulesFlat tm). 
+Definition c__makeNoneRightFlat := 5.
+Instance term_makeNoneRightFlat : computableTime' makeNoneRightFlat (fun tm _ => (1, fun q _ => (1, fun q' _ => (c__makeNoneRightFlat, fun envs _ => (makeNone_base_flat_time tm makeNoneRight_rules q q' envs, tt))))). 
+Proof. 
+  unfold makeNoneRightFlat, makeNoneRight.
+  apply computableTimeExt with (x := fun tm q q' => makeNone_base_flat tm makeNoneRight_rules q q'). 
+  1: { unfold makeNone_base_flat. easy. }
+  extract. solverec. 
+  now unfold c__makeNoneRightFlat.  
+Defined. 
+
+(** makeNoneLeft *)
+Definition makeNoneLeftFlat tm q q' := makeNoneLeft q q' (makeRulesFlat tm). 
+Definition c__makeNoneLeftFlat := 5.
+Instance term_makeNoneLeftFlat : computableTime' makeNoneLeftFlat (fun tm _ => (1, fun q _ => (1, fun q' _ => (c__makeNoneLeftFlat, fun envs _ => (makeNone_base_flat_time tm makeNoneLeft_rules q q' envs, tt))))). 
+Proof. 
+  unfold makeNoneLeftFlat, makeNoneLeft.
+  apply computableTimeExt with (x := fun tm q q' => makeNone_base_flat tm makeNoneLeft_rules q q'). 
+  1: { unfold makeNone_base_flat. easy. }
+  extract. solverec. 
+  now unfold c__makeNoneLeftFlat.  
+Defined. 
+
+(** makeNoneStay *)
+Definition makeNoneStayFlat tm q q' := makeNoneStay q q' (makeRulesFlat tm). 
+Definition c__makeNoneStayFlat := 5.
+Instance term_makeNoneStayFlat : computableTime' makeNoneStayFlat (fun tm _ => (1, fun q _ => (1, fun q' _ => (c__makeNoneStayFlat, fun envs _ => (makeNone_base_flat_time tm makeNoneStay_rules q q' envs, tt))))). 
+Proof. 
+  unfold makeNoneStayFlat, makeNoneStay.
+  apply computableTimeExt with (x := fun tm q q' => makeNone_base_flat tm makeNoneStay_rules q q'). 
+  1: { unfold makeNone_base_flat. easy. }
+  extract. solverec. 
+  now unfold c__makeNoneStayFlat.  
+Defined. 
+
+(** flat_baseEnv *)
+Definition flat_baseEnv_time (tm : TM) := makeAllEvalEnvFlat_time tm 1 0 3 0 + 17.
+Instance term_flat_baseEnv : computableTime' flat_baseEnv (fun tm _ => (flat_baseEnv_time tm, tt)). 
+Proof. 
+  extract. solverec. 
+  now unfold flat_baseEnv_time. 
+Defined.
+
+(** flat_baseEnvNone *)
+Definition flat_baseEnvNone_time (tm : TM) := makeAllEvalEnvFlat_time tm 2 2 2 0 + 23.
+Instance term_flat_baseEnvNone : computableTime' flat_baseEnvNone (fun tm _ => (flat_baseEnvNone_time tm, tt)). 
+Proof. 
+  extract. solverec. 
+  now unfold flat_baseEnvNone_time. 
+Defined.
+
+(** flat_baseEnvHalt *)
+(*Definition flat_baseEnvHalt_time (tm : TM) := makeAllEvalEnvFlat_time tm 1 0 3 0 + 17.*)
+(*Instance term_flat_baseEnvHalt : computableTime' flat_baseEnvHalt (fun tm _ => (flat_baseEnvHalt_time tm, tt)). *)
+(*Proof. *)
+  (*extract. solverec. *)
+  (*now unfold flat_baseEnvHalt_time. *)
+(*Defined.*)
+
+(** fOpt *)
+Definition c__fOpt := 8. 
+Instance term_fOpt : computableTime' fOpt (fun o _ => (c__fOpt, tt)). 
+Proof. 
+  extract. solverec. all: unfold c__fOpt; lia.
+Defined.
+
+(** opt_generateRulesForFlatNonHalt *)
+Definition c__generateRulesForFlatNonHalt := c__makeNoneLeftFlat + c__makeNoneRightFlat + c__makeNoneStayFlat + c__makeSomeLeftFlat + c__makeSomeRightFlat + c__makeSomeStayFlat + 2 * c__fOpt + 26.
+Definition generateRulesForFlatNonHalt_time (tm : TM) (q : nat) (m : option nat) (dst : nat * (option nat * TM.move)) := 
+  match m, dst with
+  | _, (q', (Some x, TM.L)) => makeSome_base_flat_time tm makeSomeRight_rules q q' (fOpt m) (fOpt $ Some x) (flat_baseEnv tm)
+  | _, (q', (Some x, TM.R)) => makeSome_base_flat_time tm makeSomeLeft_rules q q' (fOpt m) (fOpt $ Some x) (flat_baseEnv tm)
+  | _, (q', (Some x, TM.N)) => makeSome_base_flat_time tm makeSomeStay_rules q q' (fOpt m) (fOpt $ Some x) (flat_baseEnv tm)
+  | Some x, (q', (None, TM.L)) => makeSome_base_flat_time tm makeSomeRight_rules q q' (fOpt $ Some x) (fOpt $ Some x) (flat_baseEnv tm)
+  | Some x, (q', (None, TM.R)) => makeSome_base_flat_time tm makeSomeLeft_rules q q' (fOpt $ Some x) (fOpt $ Some x) (flat_baseEnv tm)
+  | Some x, (q', (None, TM.N)) => makeSome_base_flat_time tm makeSomeStay_rules q q' (fOpt $ Some x) (fOpt $ Some x) (flat_baseEnv tm)
+  | None, (q', (None, TM.L)) => makeNone_base_flat_time tm makeNoneRight_rules q q' (flat_baseEnvNone tm)
+  | None, (q', (None, TM.R)) => makeNone_base_flat_time tm makeNoneLeft_rules q q' (flat_baseEnvNone tm)
+  | None, (q', (None, TM.N)) => makeNone_base_flat_time tm makeNoneStay_rules q q' (flat_baseEnvNone tm)
+  end
+  + flat_baseEnv_time tm + flat_baseEnvNone_time tm + c__generateRulesForFlatNonHalt.
+Instance term_generateRulesForFlatNonHalt : computableTime' opt_generateRulesForFlatNonHalt (fun tm _ => (1, fun q _ => (1, fun m _ => (1, fun dst _ => (generateRulesForFlatNonHalt_time tm q m dst, tt))))). 
+Proof. 
+  apply computableTimeExt with (x:= 
+    fun tm q m transt => 
+      match m, transt with
+      | _, (q', (Some x, TM.L)) => makeSomeRightFlat tm q q' (fOpt m) (fOpt $ Some x) (flat_baseEnv tm)
+      | _, (q', (Some x, TM.R)) => makeSomeLeftFlat tm q q' (fOpt m) (fOpt $ Some x) (flat_baseEnv tm)
+      | _, (q', (Some x, TM.N)) => makeSomeStayFlat tm q q' (fOpt m) (fOpt $ Some x) (flat_baseEnv tm)
+      | Some x, (q', (None, TM.L)) => makeSomeRightFlat tm q q' (fOpt $ Some x) (fOpt $ Some x) (flat_baseEnv tm)
+      | Some x, (q', (None, TM.R)) => makeSomeLeftFlat tm q q' (fOpt $ Some x) (fOpt $ Some x) (flat_baseEnv tm)
+      | Some x, (q', (None, TM.N)) => makeSomeStayFlat tm q q' (fOpt $ Some x) (fOpt $ Some x) (flat_baseEnv tm)
+      | None, (q', (None, TM.L)) => makeNoneRightFlat tm q q' (flat_baseEnvNone tm)
+      | None, (q', (None, TM.R)) => makeNoneLeftFlat tm q q' (flat_baseEnvNone tm)
+      | None, (q', (None, TM.N)) => makeNoneStayFlat tm q q' (flat_baseEnvNone tm)
+      end). 
+  1: { unfold makeSomeLeftFlat, makeSomeStayFlat, makeSomeRightFlat, makeNoneLeftFlat, makeNoneStayFlat, makeNoneRightFlat. easy. }
+  extract. 
+  recRel_prettify2. 
+  all: unfold generateRulesForFlatNonHalt_time, c__generateRulesForFlatNonHalt. 
+  all: unfold optReturn; lia. 
+Defined. 
+
+(** inp_eqb *)
+Instance eqbComp_inp : EqBool.eqbCompT (nat * list (option nat)).
+Proof. 
+  easy.
+Defined. 
+
+Instance term_inp_eqb : computableTime' inp_eqb (fun a _ => (5, fun b _ => (@EqBool.eqbTime _ _ _ _ eqbComp_inp (size (enc a)) (size (enc b)), tt))). 
+Proof. 
+  extract. solverec. 
+Defined. 
+ 
+(** generateWindowsForFlatNonHalt *)
+From Undecidability.L.Functions Require Import FinTypeLookup EqBool.
+
+(*Print TM.*)
+(*Global Instance term_lookup :*)
+    (*computableTime' (@lookup (nat * list (option nat)) (nat * list (option nat * TM.move)) _ _) (fun x _ => (5, fun l _ => (1, fun d _ => (lookupTime (size (enc x)) l,tt)))).*)
+  (*unfold lookup. unfold eqb.*)
+  (*extract. unfold lookupTime. solverec.*)
+  (*Qed.*)
+
+Definition generateWindowsForFlatNonHalt_time (tm : TM) (q : nat) (m : option nat) := 1. 
+Instance term_generateWindowsForFlatNonHalt : computableTime' generateWindowsForFlatNonHalt (fun tm _ => (1, fun q _ => (1, fun m _ => (generateWindowsForFlatNonHalt_time tm q m, tt)))).
+Proof. 
+  unfold generateWindowsForFlatNonHalt. 
+  extract. (*TODO: extraction failing at lookup, possibly because of failing typeclass inference?*)
+
+(** halting state windows*)
+
+(**makeHalt *)
+  
+(** generateWindowsForFlatHalt *)
+Instance term_generateWindowsForFlatHalt : computableTime' generateWindowsForFlatHalt (fun tm _ => (1, fun q _ => (1, tt))). 
+Proof. 
+  apply computableTimeExt with (x := fun tm q => makeHalt
